Modest optimization of leaf functions
Leaf functions are functions that do not call any other function.  For leaf functions, it is not necessary to save the LR register on function entry nor to reload LR on function return, since LR contains the correct return address throughout the function's execution.

This commit suppresses the reloading of LR before returning from a leaf function.  LR is still saved on the stack on function entry, because doing otherwise would require extensive changes in the Stacking pass of CompCert.  However, preliminary experiments indicate that we get good speedups by avoiding to reload LR, while avoiding to save LR makes little difference in speed.

To support this optimization and its proof:
- Mach is extended with a `is_leaf_function` Boolean function and a `wf_state` predicate to provide the semantic characterization.
- Asmgenproof* is extended with a `important_preg` Boolean function that means "data register or LR".  A number of lemmas that used to show preservation of data registers now show preservation of LR as well.

backend/Mach.v
@@ -189,11 +189,17 @@ Fixpoint find_label (lbl: label) (c: code) {struct c} : option code :=
   | i1 :: il => if is_label lbl i1 then Some il else find_label lbl il
   end.
 
-Lemma find_label_incl:
-  forall lbl c c', find_label lbl c = Some c' -> incl c' c.
+Lemma find_label_tail:
+  forall lbl c c', find_label lbl c = Some c' -> is_tail c' c.
 Proof.
   induction c; simpl; intros. discriminate.
   destruct (is_label lbl a). inv H. auto with coqlib. eauto with coqlib.
+Qed.
+
+Lemma find_label_incl:
+  forall lbl c c', find_label lbl c = Some c' -> incl c' c.
+Proof.
+  intros; red; intros. eapply is_tail_incl; eauto. eapply find_label_tail; eauto.
 Qed.
 
 Section RELSEM.
@@ -426,3 +432,70 @@ Inductive final_state: state -> int -> Prop :=
 
 Definition semantics (rao: function -> code -> ptrofs -> Prop) (p: program) :=
   Semantics (step rao) (initial_state p) final_state (Genv.globalenv p).
+
+(** * Leaf functions *)
+
+(** A leaf function is a function that contains no [Mcall] instruction. *)
+
+Definition is_leaf_function (f: function) : bool :=
+  List.forallb
+    (fun i => match i with Mcall _ _ => false | _ => true end)
+    f.(fn_code).  
+
+(** Semantic characterization of leaf functions: 
+    functions in the call stack are never leaf functions. *)
+
+Section WF_STATES.
+
+Variable rao: function -> code -> ptrofs -> Prop.
+
+Variable ge: genv.
+
+Inductive wf_frame: stackframe -> Prop :=
+  | wf_stackframe_intro: forall fb sp ra c f
+        (CODE: Genv.find_funct_ptr ge fb = Some (Internal f))
+        (LEAF: is_leaf_function f = false)
+        (TAIL: is_tail c f.(fn_code)),
+      wf_frame (Stackframe fb sp ra c).
+
+Inductive wf_state: state -> Prop :=
+  | wf_normal_state: forall s fb sp c rs m f
+        (STACK: Forall wf_frame s)
+        (CODE: Genv.find_funct_ptr ge fb = Some (Internal f))
+        (TAIL: is_tail c f.(fn_code)),
+      wf_state (State s fb sp c rs m)
+  | wf_call_state: forall s fb rs m
+        (STACK: Forall wf_frame s),
+      wf_state (Callstate s fb rs m)
+  | wf_return_state: forall s rs m
+        (STACK: Forall wf_frame s),
+      wf_state (Returnstate s rs m).
+
+Lemma wf_step:
+  forall S1 t S2, step rao ge S1 t S2 -> wf_state S1 -> wf_state S2.
+Proof.
+  induction 1; intros WF; inv WF; try (econstructor; now eauto with coqlib).
+- (* call *)
+  assert (f0 = f) by congruence. subst f0.
+  constructor.
+  constructor; auto. econstructor; eauto with coqlib.
+  destruct (is_leaf_function f) eqn:E; auto.
+  unfold is_leaf_function in E; rewrite forallb_forall in E. 
+  symmetry. apply (E (Mcall sig ros)). eapply is_tail_in; eauto.
+- (* goto *)
+  assert (f0 = f) by congruence. subst f0. econstructor; eauto using find_label_tail.  
+- (* cond *)
+  assert (f0 = f) by congruence. subst f0. econstructor; eauto using find_label_tail.  
+- (* jumptable *)
+  assert (f0 = f) by congruence. subst f0. econstructor; eauto using find_label_tail.  
+- (* return *)
+  inv STACK. inv H1. econstructor; eauto.
+Qed.
+
+End WF_STATES.
+
+Lemma wf_initial:
+  forall p S, initial_state p S -> wf_state (Genv.globalenv p) S.
+Proof.
+  intros. inv H. fold ge. constructor. constructor.
+Qed.
